IMP-/Step_Semantics_Cost_Generalization/IMP_Calls_GC.thy
@@ -1,31 +1,5 @@
 
-theory IMP_Calls_GC imports "../Vars" Big_StepT_Generalized_Cost_Final begin
-
-section "IMP"
-
-text \<open>IMP with calls to IMP- programs (explicitly stored).\<close>
-datatype
-  com' = SKIP'
-      | Assign' vname aexp
-      | Seq'    com'  com'
-      | If'     vname com' com'
-      | While'  vname com'
-\<comment> \<open>The only change: A call to an IMP- @{typ com}, storing its result in the return @{typ vname}.\<close>
-      | Call'   com vname
-
-bundle com'_syntax begin
-notation Assign' ("_ ::= _" [1000, 61] 61) and
-         Seq' ("_;;/ _"  [60, 61] 60) and
-         If' ("(IF _/\<noteq>0 THEN _/ ELSE _)"  [0, 0, 61] 61) and
-         While' ("(WHILE _/\<noteq>0 DO _)"  [0, 61] 61) and
-         Call' ("CALL _ RETURN _") end
-
-bundle no_com'_syntax begin
-no_notation Assign' ("_ ::= _" [1000, 61] 61) and
-            Seq' ("_;;/ _"  [60, 61] 60) and
-            If' ("(IF _/\<noteq>0 THEN _/ ELSE _)"  [0, 0, 61] 61) and
-            While' ("(WHILE _/\<noteq>0 DO _)"  [0, 61] 61) and
-            Call' ("CALL _ RETURN _") end
+theory IMP_Calls_GC imports  "../IMP_Calls" Vars_for_GC Big_StepT_Generalized_Cost_Final begin
 
 unbundle no_com_syntax
 unbundle com'_syntax
@@ -49,13 +23,12 @@ Call': "(c,s) \<Rightarrow>\<^sub>G\<^bsup> z \<^esup> t \<Longrightarrow> (CALL
 
 text \<open>For compilation to IMP-, skip to final proof.\<close>
 
-
 declare big_step_t'_GC.intros[intro]
 
 thm big_step_t'_GC.induct
 
-lemmas big_step_t'_GC_induct  = BS_Generalized_Cost.big_step_t'_GC.induct[split_rule, OF BS_Generalized_Cost_axioms]
-
+lemmas big_step_t'_GC_induct = big_step_t'_GC.induct[split_format(complete), 
+    OF BS_Generalized_Cost_axioms, consumes 1]
 
 inductive_cases Skip'_tE[elim!]: "(SKIP',s) \<Rightarrow>\<^sub>G'\<^bsup>  x \<^esup> t"
 inductive_cases Assign'_tE[elim!]: "(x ::= a,s) \<Rightarrow>\<^sub>G'\<^bsup> p \<^esup> t"
@@ -68,20 +41,6 @@ lemma Seq'': "\<lbrakk> (c1,s1) \<Rightarrow>\<^sub>G'\<^bsup> x \<^esup> s2;  (
   by auto
 end
 
-instantiation com' :: vars
-begin
-
-fun vars_com' :: "com' \<Rightarrow> vname list" where
-"vars SKIP' = []" |
-"vars (x::=e) = x#vars e" |
-"vars (c1;;c2) = vars c1 @ vars c2" |
-"vars (IF b\<noteq>0 THEN c1 ELSE c2) = b # vars c1 @ vars c2" |
-"vars (WHILE b\<noteq>0 DO c) = b#vars c" |
-"vars (CALL c RETURN r) = r#vars c"
-
-instance ..
-
-end
 
 context BS_Generalized_Cost begin
 
@@ -159,83 +118,94 @@ qed
 
 
 lemma noninterference: 
-  "(c,s) \<Rightarrow>\<^sub>G'\<^bsup> x \<^esup> t \<Longrightarrow> set (vars c) \<subseteq> S \<Longrightarrow> s = s' on S \<Longrightarrow> \<exists>t'. (c,s') \<Rightarrow>\<^sub>G'\<^bsup> x \<^esup> t' \<and> t = t' on S"
-  sorry (* proof (induction c s x t arbitrary: s' rule: big_step_t'_induct)
-  case (Assign' x a s)
+  "(c,s) \<Rightarrow>\<^sub>G'\<^bsup> x \<^esup> t \<Longrightarrow> set (vars c) \<subseteq> S \<Longrightarrow> s = s' on S \<Longrightarrow> \<exists>t' x'. (c,s') \<Rightarrow>\<^sub>G'\<^bsup> x' \<^esup> t' \<and> t = t' on S"
+proof (induction c s x t arbitrary: s' rule: big_step_t'_GC_induct)
+  case (2 x a s)
   then show ?case 
-    using aval_eq_if_eq_on_vars big_step_t'.Assign' eq_on_def eq_on_subset fun_upd_apply set_subset_Cons vars_com'.simps(2) by fastforce
+    using aval_eq_if_eq_on_vars big_step_t'_GC.Assign' eq_on_def eq_on_subset fun_upd_apply set_subset_Cons vars_com'.simps(2) by fastforce
 next
-  case (WhileTrue' s1 b c x s2 y s3 z)
+  case (7 s1 b c C1 s2 C2 s3 C3)
   then show ?case apply auto
-    by (metis (mono_tags, lifting) WhileTrue'.hyps(1) WhileTrue'.hyps(4) big_step_t'.WhileTrue' eq_onE)
+    by (metis (mono_tags, lifting) "7.hyps"(1) "7.hyps"(4) big_step_t'_GC.WhileTrue' eq_onE)
 next
-  case (Call' c s z t r)
-  then show ?case apply auto using Vars.noninterference[of c s z t S s'] by fastforce
-qed fastforce+ *)
+  case (8 c s z t r)
+  then show ?case apply auto using noninterference[of c s z t S s'] by fastforce
+qed fastforce+
 
 lemma var'_unchanged: "(c,s) \<Rightarrow>\<^sub>G'\<^bsup>z\<^esup> t \<Longrightarrow> v \<notin> set (vars c) \<Longrightarrow> s v = t v"
-  oops
+  by (induction c s z t rule: big_step_t'_GC_induct) auto
 
 section "Inlining"
 
-subsection "Memory mapping"
-
-definition fresh :: "vname list \<Rightarrow> vname \<Rightarrow> vname" where
-  "fresh S v = CHR ''.'' # concat S @ v"
-
-lemma fresh_inj: "inj_on (fresh S) (set S)"
-  by (induction S) (auto simp: inj_on_def fresh_def)
-
-lemma fresh_len[simp]: "length (fresh S v) = Suc (length v + (\<Sum>xs\<leftarrow>S. length xs))"
-  by (induction S) (auto simp: fresh_def)
-
-lemma fresh[simp]: "fresh S v \<notin> set S"
-proof
-  have "\<forall>xs \<in> set S. length (fresh S v) > length xs"
-    by (induction S) auto
-  moreover assume "fresh S v \<in> set S"
-  ultimately show False by blast
-qed
-
-fun size\<^sub>c :: "com' \<Rightarrow> nat" where
-  "size\<^sub>c (c\<^sub>1;;c\<^sub>2) = size\<^sub>c c\<^sub>1 + size\<^sub>c c\<^sub>2" |
-  "size\<^sub>c (IF b\<noteq>0 THEN c\<^sub>1 ELSE c\<^sub>2) = size\<^sub>c c\<^sub>1 + size\<^sub>c c\<^sub>2" |
-  "size\<^sub>c (WHILE b\<noteq>0 DO c) = size\<^sub>c c" |
-  "size\<^sub>c (CALL c RETURN r) = 2 * length (vars c) + 5" |
-  "size\<^sub>c _ = 0"
-
-unbundle no_com'_syntax
-unbundle com_syntax
-
-fun ssubst where
-"ssubst m [] = SKIP" |
-"ssubst m (v#vs) = (m v) ::= A (V v) ;; ssubst m vs"
 
 fun ssubst_costs where
  "ssubst_costs m s [] = skip_costs s" |      
  "ssubst_costs m s (v#vs) = (assign_costs (A (V v)) s) + ssubst_costs m (s(m v := s v)) vs"
 
-lemma vars_ssubst[simp]: "set (vars (ssubst m vs)) = set vs \<union> m ` set vs"
-  by (induction vs) auto
+(* Feels like it shouldn't be necessary; Needs deeper analysis*)
 
-lemma lvars_ssubst[simp]: "lvars (ssubst m vs) = m ` set vs"
-  by (induction vs) auto
+inductive size\<^sub>cG :: "com' \<Rightarrow> (char list \<Rightarrow> char list) \<Rightarrow> state \<Rightarrow> nat \<Rightarrow> bool" where
+Skip'_size: "size\<^sub>cG SKIP' m s 0"|
+Assign'_size: "size\<^sub>cG (x ::= a) m s 0" |
+(* To make the predicate total. Should not be used to reason for NT programms *)
+Seq'_size_NT: "size\<^sub>cG c\<^sub>1 m s n1 \<Longrightarrow> \<forall>s' x. \<not> (c\<^sub>1,s) \<Rightarrow>\<^sub>G'\<^bsup> x \<^esup> s' \<Longrightarrow> size\<^sub>cG c\<^sub>2 m s' n2 \<Longrightarrow> size\<^sub>cG (c\<^sub>1;;c\<^sub>2) m s 0" |
+Seq'_size: "size\<^sub>cG c\<^sub>1 m s n1 \<Longrightarrow> (c\<^sub>1,s) \<Rightarrow>\<^sub>G'\<^bsup> x \<^esup> s' \<Longrightarrow> size\<^sub>cG c\<^sub>2 m s' n2 \<Longrightarrow> size\<^sub>cG (c\<^sub>1;;c\<^sub>2) m s (n1 + n2)" |
+If'_size: "size\<^sub>cG c\<^sub>1 m s n1 \<Longrightarrow> size\<^sub>cG c\<^sub>2 m s n2 \<Longrightarrow> size\<^sub>cG (IF b\<noteq>0 THEN c\<^sub>1 ELSE c\<^sub>2) m s (n1 + n2)" |
+While'_size: "size\<^sub>cG c m s n \<Longrightarrow> size\<^sub>cG (WHILE b\<noteq>0 DO c) m s n" |
+Call'_size: "size\<^sub>cG (CALL c RETURN r) m s (ssubst_costs m s (vars c))"
+
+inductive_cases Skip'_size_tE[elim!]: "size\<^sub>cG SKIP' m s n"
+inductive_cases Assign'_size_tE[elim!]: "size\<^sub>cG (x ::= a) m s n"
+inductive_cases Seq'_size_tE[elim!]: "size\<^sub>cG (c\<^sub>1;;c\<^sub>2) m s n"
+inductive_cases If'_size_tE[elim!]: "size\<^sub>cG (IF b\<noteq>0 THEN c\<^sub>1 ELSE c\<^sub>2) m s n"
+inductive_cases Call'_size_tE[elim!]: "size\<^sub>cG (CALL c RETURN r) m s n"
+inductive_cases While'_size_tE[elim]: "size\<^sub>cG (WHILE b\<noteq>0 DO c) m s n"
+
+unbundle no_com'_syntax
+unbundle com_syntax
+
+lemma size\<^sub>cG_total: "\<exists>n. size\<^sub>cG c m s n"
+proof(induction c arbitrary: s m)
+  case SKIP'
+  then show ?case 
+  using Skip'_size by auto[1]
+next
+  case (Assign' x1 x2)
+  then show ?case 
+  using Assign'_size by blast
+next
+  case (Seq' c1 c2)
+  then show ?case proof(cases "\<exists> s' x. (c1,s) \<Rightarrow>\<^sub>G'\<^bsup> x \<^esup> s'")
+    case True
+    from True obtain s' x where " (c1, s) \<Rightarrow>\<^sub>G'\<^bsup> x\<^esup>  s' " by auto
+    then show ?thesis 
+      by (meson Seq'.IH(1) Seq'.IH(2) Seq'_size)
+  next
+    case False
+    then show ?thesis 
+      using Seq'.IH(1) Seq'.IH(2) Seq'_size_NT by blast
+  qed
+next
+  case (If' x1 c1 c2)
+  then show ?case 
+    by (metis If'_size)
+next
+  case (While' x1 c)
+  then show ?case 
+    using While'_size by blast
+next
+  case (Call' x1 x2)
+  then show ?case 
+    using Call'_size by blast
+qed
 
 lemma ssubst_unchanged: "big_step_tG ((ssubst m vs),s) z t \<Longrightarrow> (\<forall>v\<in>set vs. m v \<notin> set vs) \<Longrightarrow> s = t on set vs"
-  unfolding eq_on_def using lvars_ssubst lvars_unchanged image_iff try (* by (metis (mono_tags, lifting)) *)
+  unfolding eq_on_def using lvars_ssubst lvars_unchanged image_iff 
+  by (metis (mono_tags, lifting)) 
 
 lemma ssubst_costs_correct:
  "(ssubst m vs,s) \<Rightarrow>\<^sub>G\<^bsup>z\<^esup> t \<Longrightarrow> z = ssubst_costs m s vs"
-proof (induction vs arbitrary: s)
-  case Nil
-  then show ?case by auto
-next
-  case (Cons a vs)
-  then show ?case proof-
-    have "((m a) ::= A (V a) ;; ssubst m vs, s) \<Rightarrow>\<^sub>G\<^bsup> z \<^esup> t" 
-      using Cons.prems ssubst.simps(2) by auto
-    obtain t' where 
-qed
+  by (induction m vs arbitrary: s z t rule: ssubst.induct) auto
 
 lemma ssubst_correct:
   "\<lbrakk> inj_on m (set vs); (\<forall>v\<in>set vs. m v \<notin> set vs) \<rbrakk>
@@ -248,8 +218,8 @@ next
   have 1: "(Assign (m v) (A (V v)),s) \<Rightarrow>\<^sub>G\<^bsup> assign_costs (A (V v)) s\<^esup> s(m v := s v)"
     using Assign[of _ "A (V v)"] by simp
   from Cons obtain t where
-    2: "(ssubst m vs, s(m v := s v)) \<Rightarrow>\<^sub>G\<^bsup> ssubst_costs m s vs \<^esup> t" and
-    s: "s(m v := s v) = t \<circ> m on set vs" sorry
+    2: "(ssubst m vs, s(m v := s v)) \<Rightarrow>\<^sub>G\<^bsup> ssubst_costs m (s(m v := s v)) vs \<^esup> t" and
+    s: "s(m v := s v) = t \<circ> m on set vs" by fastforce
   hence "s(m v := s v) = t \<circ> m on set (v#vs)"
   proof (cases "v\<in>set vs")
     case True then show ?thesis using s by auto
@@ -261,44 +231,39 @@ next
       using Cons.prems(1) by force
     with a have "m v \<notin> set (vars (ssubst m vs))" apply auto
       using Cons.prems(2) by force
-    hence "(s(m v := s v)) (m v) = t (m v)"  sorry (* using var_unchanged[OF 2] by blast *)
+    hence "(s(m v := s v)) (m v) = t (m v)"   using var_unchanged[OF 2] by blast
     then show ?thesis using s by auto
   qed
   hence "s = t \<circ> m on set (v # vs)"
     by (metis Cons.prems(2) eq_on_feq1 fun_upd_other list.set_intros(1))
   with 1 2 show ?case unfolding eq_on_def
-    apply (simp add: numeral_eq_Suc) sorry (*
-    by (metis One_nat_def Seq add_Suc plus_1_eq_Suc) *)
+    apply (simp add: numeral_eq_Suc) 
+    by (metis add_Suc big_step_tG.Seq)
 qed
-
 
 subsection "Command transfer"
 
-definition "transfer m c = ssubst m (vars c);;subst m c"
-
-lemma set_transfer[simp]: "set (vars (transfer m c)) = set (vars c) \<union> m ` set (vars c)"
-  unfolding transfer_def by auto
-
 lemma transfer_sound:
-  assumes c_sem: "(c,s) \<Rightarrow>\<^bsup>z\<^esup> t"
+  assumes c_sem: "(c,s) \<Rightarrow>\<^sub>G\<^bsup>z\<^esup> t"
       and s: "s = s' on set (vars c)"
       and inj: "inj_on m (set (vars c))"
       and disj: "(\<forall>v\<in>set (vars c). m v \<notin> set (vars c))"
     obtains t'
-    where "(transfer m c,s')\<Rightarrow>\<^bsup>skip_costs t' + assign_costs_of_list m s (vars c) + z\<^esup> t'"
+    where "(transfer m c,s')\<Rightarrow>\<^sub>G\<^bsup>ssubst_costs m s'(vars c) + z\<^esup> t'"
       and "t = t' o m on set (vars c)"
 proof -
   from ssubst_correct[OF inj disj] obtain s\<^sub>2 where ssubst_sem:
-    "(ssubst m (vars c),s')\<Rightarrow>\<^bsup>skip_costs s\<^sub>2 + assign_costs_of_list m s' (vars c)\<^esup> s\<^sub>2" and
-    "s' = s\<^sub>2 \<circ> m on set (vars c)"
+    "(ssubst m (vars c),s') \<Rightarrow>\<^sub>G\<^bsup>ssubst_costs m s' (vars c)\<^esup> s\<^sub>2" and
+    "s' = s\<^sub>2 \<circ> m on set (vars c)" 
     by blast
   with s have s\<^sub>2: "s = s\<^sub>2 o m on set (vars c)" by fastforce
 
   from subst_sound[OF c_sem this _ inj] obtain t' where
-    subst_sem: "(subst m c, s\<^sub>2) \<Rightarrow>\<^bsup> z \<^esup> t'" and t': "t = t' \<circ> m on set (vars c)" by auto
-  with ssubst_sem have "(transfer m c,s')\<Rightarrow>\<^bsup>skip_costs t' + assign_costs_of_list m s' (vars c) + z\<^esup> t'"
-    unfolding transfer_def sorry
-  with t' that show ?thesis sorry
+    subst_sem: "(subst m c, s\<^sub>2) \<Rightarrow>\<^sub>G\<^bsup> z \<^esup> t'" and t': "t = t' \<circ> m on set (vars c)" by auto
+  with ssubst_sem have "(transfer m c,s')\<Rightarrow>\<^sub>G\<^bsup>ssubst_costs m s' (vars c) + z\<^esup> t'"
+    unfolding transfer_def 
+    by (simp add: big_step_tG.Seq)
+  with t' that show ?thesis by blast
 qed
 
 lemma transfer_complete:
@@ -307,17 +272,16 @@ lemma transfer_complete:
       and inj: "inj_on m (set (vars c))"
       and disj: "(\<forall>v\<in>set (vars c). m v \<notin> set (vars c))"
   obtains t z
-    where "(c,s) \<Rightarrow>\<^sub>G\<^bsup>z\<^esup> t" "z' = Suc_lifted (Plus_lifted (times_lifted assign_cost  (\<lambda>x. length (vars c))) z)" "t = t' o m on set (vars c)"
+    where "(c,s) \<Rightarrow>\<^sub>G\<^bsup>z\<^esup> t" "z' = ssubst_costs m s' (vars c) + z" "t = t' o m on set (vars c)"
 proof -
   from ssubst_correct[OF inj disj] obtain s\<^sub>2' where
-     s\<^sub>2': "(ssubst m (vars c), s') \<Rightarrow>\<^bsup> Suc (2 * length (vars c)) \<^esup> s\<^sub>2'" "s' = s\<^sub>2' \<circ> m on set (vars c)"
+     s\<^sub>2': "(ssubst m (vars c), s') \<Rightarrow>\<^sub>G\<^bsup> ssubst_costs m s' (vars c) \<^esup> s\<^sub>2'" "s' = s\<^sub>2' \<circ> m on set (vars c)"
     by blast
   with transfer_sem[unfolded transfer_def] obtain z where
-   subst_sem: "(subst m c,s\<^sub>2') \<Rightarrow>\<^sub>G\<^bsup>z\<^esup> t'" and z: "z' = Suc_lifted (Plus_lifted (times_lifted assign_cost  (\<lambda>x. length (vars c))) z)"
-    using bigstep_det  sorry (* by fastforce *)
+   subst_sem: "(subst m c,s\<^sub>2') \<Rightarrow>\<^sub>G\<^bsup>z\<^esup> t'" and z: "z' = ssubst_costs m s' (vars c) + z"
+    using bigstep_det by fastforce 
   from s s\<^sub>2' have "s = s\<^sub>2' o m on set (vars c)" by fastforce 
-(*
-  from subst_complete[OF subst_sem this _ inj] that z *) show ?thesis sorry
+  from subst_complete[OF subst_sem this _ inj] that z show ?thesis by auto
 qed
 
 lemma transfer_unchanged:
@@ -330,25 +294,17 @@ proof -
     ssubst_sem: "(ssubst m (vars c),s)\<Rightarrow>\<^sub>G\<^bsup>x\<^esup> s\<^sub>2" and
     subst_sem: "(subst m c,s\<^sub>2)\<Rightarrow>\<^sub>G\<^bsup>y\<^esup> t" unfolding transfer_def by auto
   from ssubst_correct[OF inj disj] have "s = s\<^sub>2 o m on set (vars c)"
-    using \<open>(ssubst m (vars c), s) \<Rightarrow>\<^sub>G\<^bsup> x \<^esup> s\<^sub>2\<close> bigstep_det sorry
+    using \<open>(ssubst m (vars c), s) \<Rightarrow>\<^sub>G\<^bsup> x \<^esup> s\<^sub>2\<close> bigstep_det by blast
 
   have "s = s\<^sub>2 on UNIV - m ` set (vars c)"
-    using disj ssubst_sem ssubst_unchanged  sorry
+    using disj ssubst_sem ssubst_unchanged
     by (auto simp add: lvars_unchanged)
   moreover have "s\<^sub>2 = t  on UNIV - m ` set (vars c)" using var_unchanged subst_sem by auto
   ultimately show "s = t on UNIV - m ` set (vars c)" by fastforce
 qed
 
-definition "inline1 S c r =  (fresh S r) ::= A (V r);;transfer (fresh S) c;;r ::= A (V ((fresh S) r))"
-
-lemma inline1_vars_c[simp]: "set (vars c) \<subseteq> set (vars (inline1 S c r))"
-  unfolding inline1_def by auto
-
-lemma inline1_vars_r[simp]: "r \<in> set (vars (inline1 S c r))"
-  unfolding inline1_def by auto
-
 lemma inline1_unchanged:
-  assumes inline1_sem: "(inline1 S c r,s) \<Rightarrow>\<^bsup>z\<^esup> t"
+  assumes inline1_sem: "(inline1 S c r,s) \<Rightarrow>\<^sub>G\<^bsup>z\<^esup> t"
       and S: "set (r#vars c) \<subseteq> set S"
     shows "s = t on set S - {r}"
 proof -
@@ -357,11 +313,12 @@ proof -
     using S fresh fresh_inj inj_on_subset by auto
 
   from inline1_sem obtain s\<^sub>1 z\<^sub>1 z\<^sub>2  s\<^sub>2 z z\<^sub>3 where
-    to_sem: "((?m r) ::= A (V r),s) \<Rightarrow>\<^bsup>z\<^sub>1\<^esup> s\<^sub>1" and
-    "(transfer ?m c;;r ::= A (V (?m r)),s\<^sub>1)\<Rightarrow>\<^bsup>z\<^sub>2\<^esup> t" and
-    transfer_sem: "(transfer ?m c,s\<^sub>1)\<Rightarrow>\<^bsup>z\<^esup> s\<^sub>2" and
-    from_sem: "(r ::= A (V (?m r)),s\<^sub>2)\<Rightarrow>\<^bsup>z\<^sub>3\<^esup> t"
-    unfolding inline1_def by fastforce
+    to_sem: "((?m r) ::= A (V r),s) \<Rightarrow>\<^sub>G\<^bsup>z\<^sub>1\<^esup> s\<^sub>1" and
+    "(transfer ?m c;;r ::= A (V (?m r)),s\<^sub>1)\<Rightarrow>\<^sub>G\<^bsup>z\<^sub>2\<^esup> t" and
+    transfer_sem: "(transfer ?m c,s\<^sub>1)\<Rightarrow>\<^sub>G\<^bsup>z\<^esup> s\<^sub>2" and
+    from_sem: "(r ::= A (V (?m r)),s\<^sub>2)\<Rightarrow>\<^sub>G\<^bsup>z\<^sub>3\<^esup> t"
+    unfolding inline1_def apply auto
+    by (smt (verit, ccfv_threshold) Seq_costs_split big_step_tG.Seq inline1_def inline1_sem)
 
   hence s\<^sub>1: "s\<^sub>1 = s(?m r := s r)" "t = s\<^sub>2(r := s\<^sub>2(?m r))" by auto
   moreover have "s\<^sub>1 = s\<^sub>2 on set S" using transfer_unchanged[OF transfer_sem inj disj] 
@@ -373,31 +330,35 @@ proof -
 qed
 
 lemma inline1_sound:
-  assumes c_sem: "(c,s) \<Rightarrow>\<^bsup>z\<^esup> t"
+  assumes c_sem: "(c,s) \<Rightarrow>\<^sub>G\<^bsup>z\<^esup> t"
       and s: "s = s' on set (r#vars c)"
       and S: "set (r#vars c) \<subseteq> set S"
   obtains zr tr
-    where "(inline1 S c r,s') \<Rightarrow>\<^bsup>zr\<^esup> tr"
-      and "t r = tr r" "2 * length (vars c) + z + 5 = zr"
+    where "(inline1 S c r,s') \<Rightarrow>\<^sub>G\<^bsup>zr\<^esup> tr"
+      and "t r = tr r" "assign_costs (A (V r)) s' +
+               (ssubst_costs (fresh S) (s'(fresh S r := s' r)) (vars c) + z) +
+               assign_costs (A (V r)) t = zr"
 proof -
-  let ?m = "fresh S" let ?s\<^sub>1' = "s'((?m r) := s' r)" let ?z' = "Suc (2 * length (vars c)) + z"
+  let ?m = "fresh S" let ?s\<^sub>1' = "s'((?m r) := s' r)" let ?z' = "ssubst_costs ?m ?s\<^sub>1' (vars c) + z"
 
   have inj: "inj_on ?m (set (vars c))" using S fresh_inj inj_on_subset by auto
   have disj: "(\<forall>v\<in>set (vars c). ?m v \<notin> set (vars c))" using S fresh by auto
 
-  have 1: "((?m r) ::= A (V r),s') \<Rightarrow>\<^bsup>Suc (Suc 0)\<^esup> ?s\<^sub>1'"
-    using big_step_t.Assign[of "?m r" "A (V r)" s'] by auto
+  have 1: "((?m r) ::= A (V r),s') \<Rightarrow>\<^sub>G\<^bsup>assign_costs (A (V r)) s'\<^esup> ?s\<^sub>1'"
+    using big_step_tG.Assign[of "?m r" "A (V r)" s'] by auto
   have s\<^sub>1': "s = ?s\<^sub>1' on set (vars c)" using S s by fastforce
 
+
+
   obtain s\<^sub>2' where
-    2: "(transfer ?m c, ?s\<^sub>1') \<Rightarrow>\<^bsup>?z'\<^esup> s\<^sub>2'" and s\<^sub>2': "t = s\<^sub>2' \<circ> ?m on set (vars c)"
+    2: "(transfer ?m c, ?s\<^sub>1') \<Rightarrow>\<^sub>G\<^bsup>?z'\<^esup> s\<^sub>2'" and s\<^sub>2': "t = s\<^sub>2' \<circ> ?m on set (vars c)"
     using transfer_sound[OF c_sem s\<^sub>1' inj disj] by blast
 
   then obtain tr where
-    3: "(r ::= A (V (?m r)),s\<^sub>2')\<Rightarrow>\<^bsup>Suc (Suc 0)\<^esup> tr" and tr: "tr = s\<^sub>2'(r := s\<^sub>2'(?m r))"
-    by fastforce
+    3: "(r ::= A (V (?m r)),s\<^sub>2') \<Rightarrow>\<^sub>G\<^bsup> assign_costs (A (V (?m r))) s\<^sub>2'\<^esup> tr" and tr: "tr = s\<^sub>2'(r := s\<^sub>2'(?m r))"
+    using big_step_tG.Assign[of r "A (V (?m r))" s\<^sub>2'] by auto
 
-  from 1 2 3 s\<^sub>1' have res: "(inline1 S c r,s')\<Rightarrow>\<^bsup>Suc (Suc 0) + ?z' + Suc (Suc 0)\<^esup> tr"
+  from 1 2 3 s\<^sub>1' have res: "(inline1 S c r,s')\<Rightarrow>\<^sub>G\<^bsup>assign_costs (A (V r)) s' + ?z' + assign_costs (A (V (?m r))) s\<^sub>2'\<^esup> tr"
     unfolding inline1_def using Seq by meson
 
   have "t r = tr r"
@@ -415,39 +376,48 @@ proof -
 
     then show ?thesis using s tr c_sem False var_unchanged by fastforce
   qed
-  then show ?thesis using that res by auto
+  have "assign_costs (A (V r)) t = assign_costs ((subst ?m (A (V r)))) s\<^sub>2'"
+    using subst_costs_assign 
+    using \<open>t r = tr r\<close> tr by force
+  hence ascs: "assign_costs (A (V r)) t = assign_costs (A (V (fresh S r))) s\<^sub>2'"
+    by simp
+  then show ?thesis using that res ascs 
+    using \<open>t r = tr r\<close> by auto
 qed
 
 lemma inline1_complete:
-  assumes inline_sem: "(inline1 S c r,s') \<Rightarrow>\<^bsup>zr\<^esup> tr"
+  assumes inline_sem: "(inline1 S c r,s') \<Rightarrow>\<^sub>G\<^bsup>zr\<^esup> tr"
       and s: "s = s' on set (r#vars c)"
       and S: "set (r#vars c) \<subseteq> set S"
   obtains z t
-    where "(c,s) \<Rightarrow>\<^bsup>z\<^esup> t \<and> tr r = t r \<and> 2 * length (vars c) + z + 5 = zr"
+    where "(c,s) \<Rightarrow>\<^sub>G\<^bsup>z\<^esup> t \<and> tr r = t r \<and> assign_costs (A (V r)) s' +
+               (ssubst_costs (fresh S) (s'(fresh S r := s' r)) (vars c) + z) +
+               assign_costs (A (V r)) tr = zr"
 proof -
   let ?m = "fresh S" let ?s\<^sub>1' = "s'((?m r) := s' r)"
 
   have inj: "inj_on ?m (set (vars c))" using S fresh_inj inj_on_subset by auto
   have disj: "(\<forall>v\<in>set (vars c). ?m v \<notin> set (vars c))" using S fresh by auto
 
-  have 1: "((?m r) ::= A (V r),s') \<Rightarrow>\<^bsup>Suc (Suc 0)\<^esup> ?s\<^sub>1'"
-    using big_step_t.Assign[of "?m r" "A (V r)" s'] by auto
+  have 1: "((?m r) ::= A (V r),s') \<Rightarrow>\<^sub>G\<^bsup>assign_costs (A (V r)) s'\<^esup> ?s\<^sub>1'"
+    using big_step_tG.Assign[of "?m r" "A (V r)" s'] by auto
   have s\<^sub>1': "?s\<^sub>1' = s on set (vars c)" using S s by fastforce
 
   from inline_sem obtain t' z' where
-    2: "(transfer ?m c,?s\<^sub>1') \<Rightarrow>\<^bsup>z'\<^esup> t'" and z': "z' + 4 = zr"
+    2: "(transfer ?m c,?s\<^sub>1') \<Rightarrow>\<^sub>G\<^bsup>z'\<^esup> t'" and z': "assign_costs (A (V r)) s' + z' + assign_costs (A (V r)) tr = zr"
     unfolding inline1_def by fastforce
   from transfer_complete[OF 2 s\<^sub>1' inj disj] obtain t z where
-    c_sem: "(c, s) \<Rightarrow>\<^bsup> z \<^esup> t" and
-    z: "z' = Suc (2 * length (vars c)) + z" and
+    c_sem: "(c, s)  \<Rightarrow>\<^sub>G\<^bsup>z\<^esup> t" and
+    z: "z' = ssubst_costs (fresh S) (s'(fresh S r := s' r)) (vars c) + z" and
     t: "t = t' \<circ> fresh S on set (vars c)" by metis
 
   obtain tr' where
-    3: "(r ::= A (V (?m r)),t')\<Rightarrow>\<^bsup>Suc (Suc 0)\<^esup> tr'" and tr: "tr' = t'(r := t'(?m r))"
-    by fastforce
+    3: "(r ::= A (V (?m r)),t')\<Rightarrow>\<^sub>G\<^bsup>assign_costs (A (V (?m r))) t'\<^esup> tr'" and tr: "tr' = t'(r := t'(?m r))"
+    using big_step_tG.Assign[of r "A (V (?m r))" t'] by auto
 
-  moreover from z have "(inline1 S c r,s')\<Rightarrow>\<^bsup>Suc (Suc 0) + Suc (2 * length (vars c)) + z + Suc (Suc 0)\<^esup> tr'"
-    unfolding inline1_def using Seq[OF 1 2] Seq[OF _ 3] by auto
+  moreover from z have "(inline1 S c r,s')\<Rightarrow>\<^sub>G\<^bsup>assign_costs (A (V r)) s' + ssubst_costs ?m ?s\<^sub>1' (vars c) + z + assign_costs (A (V (?m r))) t'\<^esup> tr'"
+    unfolding inline1_def using Seq[OF 1 2] Seq[OF _ 3] 
+    by (metis (no_types, lifting) add.assoc)
 
   ultimately have tr': "tr' = tr"
     using bigstep_det inline_sem by blast
@@ -471,63 +441,314 @@ proof -
   then show ?thesis using that c_sem z z' tr' by auto
 qed
 
-
 section \<open>Program inlining\<close>
 
-fun inline_S :: "vname list \<Rightarrow> com' \<Rightarrow> com" where
-  "inline_S S SKIP' = SKIP" |
-  "inline_S S (Assign' x a) = (x::=a)" |
-  "inline_S S (Seq' c\<^sub>1' c\<^sub>2') = inline_S S c\<^sub>1';;inline_S S c\<^sub>2'" |
-  "inline_S S (If' b c\<^sub>1' c\<^sub>2') = IF b\<noteq>0 THEN inline_S S c\<^sub>1' ELSE inline_S S c\<^sub>2'" |
-  "inline_S S (While' b c') = WHILE b\<noteq>0 DO inline_S S c'" |
-  "inline_S S (Call' c r) = inline1 S c r"
-
-lemma vars_inline_S[simp]: "set (vars c) \<subseteq> set (vars (inline_S S c))"
-  by (induction c arbitrary: S) auto
-
-lemma inline_S_sound:
-  "\<lbrakk> (c',s') \<Rightarrow>'\<^bsup>z'\<^esup> t'; s'= s on set S; set (vars c') \<subseteq> set S \<rbrakk>
-    \<Longrightarrow> \<exists>t z. (inline_S S c',s)\<Rightarrow>\<^bsup>z\<^esup> t \<and> t = t' on set S \<and> z' \<le> z \<and> z \<le> z' + (z' + 1) * size\<^sub>c c'"
-proof(induction c' s' z' t' arbitrary: s rule: big_step_t'_induct)
-  case (Assign' x a s' s)
-  hence "s(x := aval a s) = s'(x := aval a s') on set S"
-    unfolding eq_on_def apply auto
-    by (metis Assign'.prems(1) aval_eq_if_eq_on_vars eq_on_subset)
-  moreover have "(inline_S S (Assign' x a), s) \<Rightarrow>\<^bsup> Suc (Suc 0) \<^esup> s(x := aval a s)" by auto
-  ultimately show ?case by fastforce
+lemma inline_S_sound_costs_lb: 
+  "\<lbrakk>(c',s') \<Rightarrow>\<^sub>G'\<^bsup>z'\<^esup> t'; size\<^sub>cG c' (fresh S) s' n; s'= s on set S; set (vars c') \<subseteq> set S\<rbrakk>
+    \<Longrightarrow> \<exists>t z. (inline_S S c',s) \<Rightarrow>\<^sub>G\<^bsup>z\<^esup> t \<and> t = t' on set S \<and> z' \<le> z"
+proof(induction c' s' z' t' arbitrary:  n s rule: big_step_t'_GC_induct)
+  case (1 s)
+  then show ?case sorry
 next
-  case (Seq' c\<^sub>1 s\<^sub>1 x s\<^sub>2 c\<^sub>2 y s\<^sub>3 z s\<^sub>1')
-  then obtain s\<^sub>2' x' where
-    1: "(inline_S S c\<^sub>1, s\<^sub>1') \<Rightarrow>\<^bsup> x' \<^esup> s\<^sub>2' \<and> s\<^sub>2' = s\<^sub>2 on set S \<and> x \<le> x' \<and> x' \<le> x + (x + 1) * size\<^sub>c c\<^sub>1"
+  case (2 x a s')
+  have  "(x ::= a, s) \<Rightarrow>\<^sub>G\<^bsup> assign_costs a s \<^esup> s(x := aval a s)" 
+    using big_step_tG.Assign by auto
+  hence 1: "(inline_S S (Assign' x a), s) \<Rightarrow>\<^sub>G\<^bsup> assign_costs a s \<^esup> s(x := aval a s)"
+    by auto
+  from \<open>set (vars (Assign' x a)) \<subseteq> set S\<close> have "set (vars a) \<subseteq> set S" by auto
+  hence  "assign_costs a s = assign_costs a s'" using assign_costs_noninterference 
+    using "2.prems"(2) 
+    using "2.prems"(1) 
+    by simp
+  hence 2: "assign_costs a s' \<le> assign_costs a s  \<and> assign_costs a s  \<le> assign_costs a s'"
+    by simp
+  from \<open>set (vars a) \<subseteq> set S\<close> have 3: "s(x := aval a s) = s'(x := aval a s') on set S"
+    using "2.prems"(2) "2.prems"(3) local.noninterference 
+    using "2.prems"(1) 
     by fastforce
-  hence prems2: "s\<^sub>2 = s\<^sub>2' on set S" by fastforce
-  from Seq' obtain s\<^sub>3' y' where
-    2: "(inline_S S c\<^sub>2, s\<^sub>2') \<Rightarrow>\<^bsup> y' \<^esup> s\<^sub>3' \<and> s\<^sub>3' = s\<^sub>3 on set S \<and> y \<le> y' \<and> y' \<le> y + (y + 1) * size\<^sub>c c\<^sub>2"
-    using Seq'.IH(2)[OF prems2] by auto
-  from 1 2 Seq'.hyps(3) show ?case by (fastforce simp: algebra_simps)
+  from 1 2 3 show ?case 
+    by (metis "2.prems"(2) "2.prems"(3) Assign'_tE \<open>(x ::= a, s) \<Rightarrow>\<^sub>G\<^bsup> assign_costs a s \<^esup> s (x := aval a s)\<close> \<open>set (vars a) \<subseteq> set S\<close> aexp_costs_noninterference local.Assign_tE)
 next
-  case (WhileTrue' s\<^sub>1 b c\<^sub>1 x s\<^sub>2 y s\<^sub>3 z s\<^sub>1')
-  hence prems1: "set (vars c\<^sub>1) \<subseteq> set S" by simp
-  obtain s\<^sub>2' x' where 1: "(inline_S S c\<^sub>1, s\<^sub>1') \<Rightarrow>\<^bsup> x' \<^esup> s\<^sub>2' \<and> s\<^sub>2' = s\<^sub>2 on set S \<and> x \<le> x' \<and> x' \<le> x + (x + 1) * size\<^sub>c c\<^sub>1"
-    using WhileTrue'.IH(1)[OF WhileTrue'.prems(1) prems1] by blast
-  with WhileTrue' have prems2: "s\<^sub>2 = s\<^sub>2' on set S" "set (vars (While' b c\<^sub>1)) \<subseteq> set S" by auto
-  obtain s\<^sub>3' y' where 2: "(inline_S S (While' b c\<^sub>1), s\<^sub>2') \<Rightarrow>\<^bsup> y' \<^esup> s\<^sub>3' \<and> s\<^sub>3' = s\<^sub>3 on set S \<and> y \<le> y' \<and> y' \<le> y + (y + 1) * size\<^sub>c (While' b c\<^sub>1)"
-    using WhileTrue'.IH(2)[OF prems2] by auto
-  from WhileTrue' have "s\<^sub>1' b \<noteq> 0" by auto
-  with 1 2 WhileTrue'.hyps(4) have "(inline_S S (While' b c\<^sub>1), s\<^sub>1') \<Rightarrow>\<^bsup> 1 + x' + y' \<^esup> s\<^sub>3' \<and> s\<^sub>3' = s\<^sub>3 on set S \<and> z \<le> 1 + x' + y' \<and> 1 + x' + y' \<le> z + (z + 1) * size\<^sub>c (While' b c\<^sub>1)"
+  case (3 c1 s1 C1 s2 c2 C2 s3 C3)
+  from \<open>set (vars (Seq' c1 c2)) \<subseteq> set S\<close> have "set (vars c1) \<subseteq> set S" "set (vars c2) \<subseteq> set S"
+    by simp+
+  from \<open>size\<^sub>cG (Seq' c1 c2) (fresh S) s1 n\<close> \<open>(c1, s1) \<Rightarrow>\<^sub>G'\<^bsup> C1\<^esup>  s2\<close> obtain n1 n2 where
+      "size\<^sub>cG c1 (fresh S) s1 n1" "size\<^sub>cG c2 (fresh S) s2 n2" "n = n1 + n2"
+    using BS_Generalized_Cost.state_determ BS_Generalized_Cost_axioms by blast
+  from "3.IH"(1)[OF \<open>size\<^sub>cG c1 (fresh S) s1 n1\<close> \<open>s1 = s on set S\<close> \<open>set (vars c1) \<subseteq> set S\<close>]
+  obtain t1 z1 where "(inline_S S c1, s) \<Rightarrow>\<^sub>G\<^bsup> z1 \<^esup> t1 " "t1 = s2 on set S" " C1 \<le> z1" 
+    by auto
+  have \<open>s2 = t1 on set S\<close> 
+    using \<open>t1 = s2 on set S\<close> by auto
+  from "3.IH"(2)[OF \<open>size\<^sub>cG c2 (fresh S) s2 n2\<close> \<open>s2 = t1 on set S\<close> \<open>set (vars c2) \<subseteq> set S\<close>]
+  obtain t2 z2 where "(inline_S S c2, t1) \<Rightarrow>\<^sub>G\<^bsup> z2 \<^esup> t2 " " t2 = s3 on set S " "C2 \<le> z2"
+    by blast
+  have "(Seq (inline_S S c1) (inline_S S c2), s) \<Rightarrow>\<^sub>G\<^bsup> z1 + z2 \<^esup> t2"
+    using BS_Generalized_Cost_axioms \<open>(inline_S S c1, s) \<Rightarrow>\<^sub>G\<^bsup> z1 \<^esup> t1\<close> \<open>(inline_S S c2, t1) \<Rightarrow>\<^sub>G\<^bsup> z2 \<^esup> t2\<close> by blast
+  hence "(inline_S S (Seq' c1  c2), s) \<Rightarrow>\<^sub>G\<^bsup> z1 + z2 \<^esup> t2" by auto
+  have "C1 + C2 \<le> z1 + z2"
+    using \<open>C1 \<le> z1\<close> \<open>C2 \<le> z2\<close> by simp
+  hence "C1 + C2 \<le> z1 + z2"
+    by simp
+  hence "C3 \<le> z1 + z2 "
+    using \<open>C3 = C1 + C2\<close> 
+    by simp
+  hence "C3 \<le> z1 + z2"
+    by simp
+  hence "C3 \<le> z1 + z2"
     by (auto simp: algebra_simps)
-  thus ?case by blast
+  hence "C3 \<le> z1 + z2"
+    using \<open>C3 = C1 + C2\<close> by (auto simp: algebra_simps)
+  hence "C3 \<le> z1 + z2"
+    using \<open>C3 = C1 + C2\<close> by (auto simp: algebra_simps)
+  then show ?case 
+    using \<open>(inline_S S (Seq' c1 c2), s) \<Rightarrow>\<^sub>G\<^bsup> z1 + z2 \<^esup> t2\<close> \<open>(inline_S S c2, t1) \<Rightarrow>\<^sub>G\<^bsup> z2 \<^esup> t2\<close> \<open>t2 = s3 on set S\<close> by blast
 next
-  case (Call' c s z t r s')
-  hence prems: "s = s' on set (r # vars c)" "set (r # vars c) \<subseteq> set S" by auto
+  case (4 s' b c1 C t C' c2)
+  from \<open>size\<^sub>cG (If' b c1 c2) (fresh S) s' n\<close> obtain n1 n2 x'  where
+      "size\<^sub>cG c1 (fresh S) s' n1""size\<^sub>cG c2 (fresh S) s' n2" "n = n1 + n2"
+    by auto
+  from \<open>set (vars (If' b c1 c2)) \<subseteq> set S\<close> have "set (vars c1) \<subseteq> set S" "set (vars c2) \<subseteq> set S"
+    by simp+have "b \<in> set S" 
+     using \<open>set (vars (If' b c1 c2)) \<subseteq> set S\<close> by fastforce 
+   hence "s b \<noteq> 0" 
+     using \<open>s' = s on set S\<close> \<open>s' b \<noteq> 0\<close> by auto
+  from "4.IH"[OF \<open>size\<^sub>cG c1 (fresh S) s' n1 \<close> \<open>s' = s on set S\<close> \<open>set (vars c1) \<subseteq> set S\<close>] 
+  obtain t2 z2 where "(inline_S S c1, s) \<Rightarrow>\<^sub>G\<^bsup> z2 \<^esup> t2 " "t2 = t on set S " "C \<le> z2"
+    by auto 
+  from IfTrue[of s b "(inline_S S c1)" z2 t2 _ "(inline_S S c2)"]
+  have 1: "(If b (inline_S S c1) (inline_S S c2), s) \<Rightarrow>\<^sub>G\<^bsup> z2 + 1\<^esup> t2" 
+    using \<open>s b \<noteq> 0 \<close> \<open>(inline_S S c1, s) \<Rightarrow>\<^sub>G\<^bsup> z2 \<^esup> t2\<close>
+    by (simp add: big_step_tG.IfTrue)
+  have "Suc C \<le> Suc z2"
+    using \<open>C \<le> z2\<close> by auto
+  hence "C' \<le> Suc z2"
+    by (simp add: \<open>C' = Suc C\<close>)
+  hence "C' \<le> Suc z2"
+    by (auto simp: algebra_simps)
+  hence 3: "C' \<le> Suc z2"
+    using \<open>n = n1 + n2\<close> by auto
+  from 1 3  show ?case 
+    by (metis Suc_eq_plus1 \<open>t2 = t on set S\<close> inline_S.simps(4))
+next
+  case (5 s' b c2 C t C' c1)
+  from \<open>size\<^sub>cG (If' b c1 c2) (fresh S) s' n\<close> obtain n1 n2 x'  where
+      "size\<^sub>cG c1 (fresh S) s' n1""size\<^sub>cG c2 (fresh S) s' n2" "n = n1 + n2"
+    by auto
+  from \<open>set (vars (If' b c1 c2)) \<subseteq> set S\<close> have "set (vars c1) \<subseteq> set S" "set (vars c2) \<subseteq> set S"
+    by simp+have "b \<in> set S" 
+     using \<open>set (vars (If' b c1 c2)) \<subseteq> set S\<close> by fastforce 
+   hence "s b = 0" 
+     using \<open>s' = s on set S\<close> \<open>s' b = 0\<close> by auto
+  from "5.IH"[OF \<open>size\<^sub>cG c2 (fresh S) s' n2 \<close> \<open>s' = s on set S\<close> \<open>set (vars c2) \<subseteq> set S\<close>] 
+  obtain t2 z2 where "(inline_S S c2, s) \<Rightarrow>\<^sub>G\<^bsup> z2 \<^esup> t2 " "t2 = t on set S " "C \<le> z2"
+    by auto 
+  from IfFalse[of s b "(inline_S S c1)" z2 t2 _ "(inline_S S c2)"]
+  have 1: "(If b (inline_S S c1) (inline_S S c2), s) \<Rightarrow>\<^sub>G\<^bsup> z2 + 1\<^esup> t2" 
+    using \<open>s b = 0 \<close> \<open>(inline_S S c2, s) \<Rightarrow>\<^sub>G\<^bsup> z2 \<^esup> t2\<close>
+    by (simp add: big_step_tG.IfFalse)
+  have "Suc C \<le> Suc z2"
+    using \<open>C \<le> z2\<close> by auto
+  hence "C' \<le> Suc z2"
+    by (simp add: \<open>C' = Suc C\<close>)
+  hence "C' \<le> Suc z2"
+    by (auto simp: algebra_simps)
+  hence 3: "C' \<le> Suc z2"
+    using \<open>n = n1 + n2\<close> by auto
+  from 1 3  show ?case 
+    by (metis Suc_eq_plus1 \<open>t2 = t on set S\<close> inline_S.simps(4))
+next
+  case (6 s b c)
+  then show ?case sorry
+next
+  case (7 s1 b c C1 s2 C2 s3 C3)
+  from \<open>s1 b \<noteq> 0\<close> \<open>set (vars (While' b c)) \<subseteq> set S\<close> \<open> s1 = s on set S\<close> have \<open>s b \<noteq> 0\<close> by auto
+  from \<open>set (vars (While' b c)) \<subseteq> set S\<close> have \<open>set (vars c) \<subseteq> set S\<close> by auto
+  from \<open>size\<^sub>cG (While' b c) (fresh S) s1 n\<close> have \<open>size\<^sub>cG c (fresh S) s1 n\<close> by auto
+  obtain n2 where "size\<^sub>cG (While' b c) (fresh S) s2 n2"
+    using size\<^sub>cG_total by blast
+  from "7.IH"(1)[OF \<open>size\<^sub>cG c (fresh S) s1 n\<close> \<open>s1 = s on set S\<close> \<open>set (vars c) \<subseteq> set S\<close>]
+  obtain C1' s2' where 1: \<open>(inline_S S c, s) \<Rightarrow>\<^sub>G\<^bsup> C1' \<^esup> s2' \<close>\<open> s2' = s2 on set S \<close> \<open> C1 \<le> C1'\<close> by auto
+  hence \<open>s2 = s2' on set S\<close> by auto
+  from "7.IH"(2)[OF \<open>size\<^sub>cG (While' b c) (fresh S) s2 n2\<close> \<open>s2 = s2' on set S\<close> \<open>set (vars (While' b c)) \<subseteq> set S\<close>]
+  obtain C2' s3' where 2: \<open>(inline_S S (While' b c), s2') \<Rightarrow>\<^sub>G\<^bsup> C2' \<^esup> s3' \<close>\<open> s3' = s3 on set S \<close> \<open>C2 \<le> C2'\<close> by auto
+  hence \<open>((While b (inline_S S c)), s2') \<Rightarrow>\<^sub>G\<^bsup> C2' \<^esup> s3'\<close> by auto
+  from \<open>(inline_S S c, s) \<Rightarrow>\<^sub>G\<^bsup> C1' \<^esup> s2' \<close> \<open>((While b (inline_S S c)), s2') \<Rightarrow>\<^sub>G\<^bsup> C2' \<^esup> s3'\<close>  \<open>s b \<noteq> 0\<close>
+  have \<open>((While b (inline_S S c)), s) \<Rightarrow>\<^sub>G\<^bsup> C1' + C2' + 1 \<^esup> s3'\<close> 
+    by (simp add: big_step_tG.WhileTrue)
+  hence \<open>(inline_S S (While' b c), s)  \<Rightarrow>\<^sub>G\<^bsup> C1' + C2' + 1 \<^esup> s3'\<close> by auto    
+  from \<open>C1 \<le> C1'\<close> \<open>C2 \<le> C2'\<close> \<open>C1 + C2 + 1 = C3\<close> have "C3 \<le> C1' + C2' + 1" by simp 
+  from \<open>(inline_S S (While' b c), s)  \<Rightarrow>\<^sub>G\<^bsup> C1' + C2' + 1 \<^esup> s3'\<close> \<open> s3' = s3 on set S\<close> \<open>C3 \<le> C1' + C2' + 1\<close> show ?case
+    by auto
+next
+  case (8 c s' z t r)
+  hence prems: "s' = s on set (r # vars c)" "set (r # vars c) \<subseteq> set S" 
+    using eq_onI eq_on_subset vars_com'.simps(6) by fastforce+
+
   then obtain zr tr where
-    inline: "(inline1 S c r, s') \<Rightarrow>\<^bsup> zr \<^esup> tr" "t r = tr r" "2 * length (vars c) + z + 5 = zr"
-    using inline1_sound[OF Call'.hyps] by blast
-  with Call'.prems(1) inline1_unchanged[OF inline(1) prems(2)] have "tr = s(r := tr r) on set S"
-    by fastforce
-  with inline have " (inline_S S (Call' c r), s') \<Rightarrow>\<^bsup> zr \<^esup> tr \<and> tr = s(r := t r) on set S \<and> z \<le> zr \<and> zr \<le> z + (z + 1) * size\<^sub>c (Call' c r)" by simp
+    inline: "(inline1 S c r, s) \<Rightarrow>\<^sub>G\<^bsup>  zr \<^esup> tr" "t r = tr r" 
+    "assign_costs (A (V r)) s + (ssubst_costs (fresh S) (s(fresh S r := s r)) (vars c) + z) +
+               assign_costs (A (V r)) t = zr"
+    using inline1_sound[OF \<open>(c, s') \<Rightarrow>\<^sub>G\<^bsup> z \<^esup> t\<close> \<open>s' = s on set (r # vars c)\<close> \<open>set (r # vars c) \<subseteq> set S\<close>] by auto
+  with "8.prems"(1) inline1_unchanged[OF inline(1) prems(2)] have "tr = s'(r := tr r) on set S"
+    using "8.prems"(2) fun_upd_apply by fastforce
+  with inline have " (inline_S S (Call' c r), s) \<Rightarrow>\<^sub>G\<^bsup>  zr \<^esup> tr \<and> tr = s'(r := t r) on set S \<and> z \<le> zr" by simp
   then show ?case by blast
-qed (auto | (fastforce simp: algebra_simps))+
+qed
+
+lemma inline_S_sound_costs_lb: 
+  "\<lbrakk>(c',s') \<Rightarrow>\<^sub>G'\<^bsup>z'\<^esup> t'; size\<^sub>cG c' (fresh S) s' n; s'= s on set S; set (vars c') \<subseteq> set S\<rbrakk>
+    \<Longrightarrow> \<exists>t z. (inline_S S c',s) \<Rightarrow>\<^sub>G\<^bsup>z\<^esup> t \<and> t = t' on set S \<and> z \<le> z' + (z' + 1) * n"
+proof(induction c' s' z' t' arbitrary:  n s rule: big_step_t'_GC_induct)
+  case (1 s)
+  then show ?case sorry
+next
+  case (2 x a s')
+  have  "(x ::= a, s) \<Rightarrow>\<^sub>G\<^bsup> assign_costs a s \<^esup> s(x := aval a s)" 
+    using big_step_tG.Assign by auto
+  hence 1: "(inline_S S (Assign' x a), s) \<Rightarrow>\<^sub>G\<^bsup> assign_costs a s \<^esup> s(x := aval a s)"
+    by auto
+  from \<open>set (vars (Assign' x a)) \<subseteq> set S\<close> have "set (vars a) \<subseteq> set S" by auto
+  hence  "assign_costs a s = assign_costs a s'" using assign_costs_noninterference 
+    using "2.prems"(2) 
+    using "2.prems"(1) 
+    by simp
+  hence 2: "assign_costs a s' \<le> assign_costs a s  \<and> assign_costs a s  \<le> assign_costs a s'"
+    by simp
+  from \<open>set (vars a) \<subseteq> set S\<close> have 3: "s(x := aval a s) = s'(x := aval a s') on set S"
+    using "2.prems"(2) "2.prems"(3) local.noninterference 
+    using "2.prems"(1) 
+    by fastforce
+  from 1 2 3 show ?case 
+    by (metis \<open>assign_costs a s = assign_costs a s'\<close> le_add1)
+next
+  case (3 c1 s1 C1 s2 c2 C2 s3 C3)
+  from \<open>set (vars (Seq' c1 c2)) \<subseteq> set S\<close> have "set (vars c1) \<subseteq> set S" "set (vars c2) \<subseteq> set S"
+    by simp+
+  from \<open>size\<^sub>cG (Seq' c1 c2) (fresh S) s1 n\<close> \<open>(c1, s1) \<Rightarrow>\<^sub>G'\<^bsup> C1\<^esup>  s2\<close> obtain n1 n2 where
+      "size\<^sub>cG c1 (fresh S) s1 n1" "size\<^sub>cG c2 (fresh S) s2 n2" "n = n1 + n2"
+    using BS_Generalized_Cost.state_determ BS_Generalized_Cost_axioms by blast
+  from "3.IH"(1)[OF \<open>size\<^sub>cG c1 (fresh S) s1 n1\<close> \<open>s1 = s on set S\<close> \<open>set (vars c1) \<subseteq> set S\<close>]
+  obtain t1 z1 where "(inline_S S c1, s) \<Rightarrow>\<^sub>G\<^bsup> z1 \<^esup> t1 " "t1 = s2 on set S" " z1 \<le> C1 + (C1 + 1) * n1" 
+    by auto
+  have \<open>s2 = t1 on set S\<close> 
+    using \<open>t1 = s2 on set S\<close> by auto
+  from "3.IH"(2)[OF \<open>size\<^sub>cG c2 (fresh S) s2 n2\<close> \<open>s2 = t1 on set S\<close> \<open>set (vars c2) \<subseteq> set S\<close>]
+  obtain t2 z2 where "(inline_S S c2, t1) \<Rightarrow>\<^sub>G\<^bsup> z2 \<^esup> t2 " " t2 = s3 on set S " "z2 \<le> C2 + (C2 + 1) * n2"
+    by blast
+  have "(Seq (inline_S S c1) (inline_S S c2), s) \<Rightarrow>\<^sub>G\<^bsup> z1 + z2 \<^esup> t2"
+    using BS_Generalized_Cost_axioms \<open>(inline_S S c1, s) \<Rightarrow>\<^sub>G\<^bsup> z1 \<^esup> t1\<close> \<open>(inline_S S c2, t1) \<Rightarrow>\<^sub>G\<^bsup> z2 \<^esup> t2\<close> by blast
+  hence "(inline_S S (Seq' c1  c2), s) \<Rightarrow>\<^sub>G\<^bsup> z1 + z2 \<^esup> t2" by auto
+  have "C1 + C2 \<le> z1 + z2"
+    using \<open>C1 \<le> z1\<close> \<open>C2 \<le> z2\<close> by simp
+  hence "C1 + C2 \<le> z1 + z2"
+    by simp
+  hence "C3 \<le> z1 + z2 "
+    using \<open>C3 = C1 + C2\<close> 
+    by simp
+  hence "C3 \<le> z1 + z2"
+    by simp
+  hence "C3 \<le> z1 + z2"
+    by (auto simp: algebra_simps)
+  hence "C3 \<le> z1 + z2"
+    using \<open>C3 = C1 + C2\<close> by (auto simp: algebra_simps)
+  hence "C3 \<le> z1 + z2"
+    using \<open>C3 = C1 + C2\<close> by (auto simp: algebra_simps)
+  then show ?case 
+    using \<open>(inline_S S (Seq' c1 c2), s) \<Rightarrow>\<^sub>G\<^bsup> z1 + z2 \<^esup> t2\<close> \<open>(inline_S S c2, t1) \<Rightarrow>\<^sub>G\<^bsup> z2 \<^esup> t2\<close> \<open>t2 = s3 on set S\<close> by blast
+next
+  case (4 s' b c1 C t C' c2)
+  from \<open>size\<^sub>cG (If' b c1 c2) (fresh S) s' n\<close> obtain n1 n2 x'  where
+      "size\<^sub>cG c1 (fresh S) s' n1""size\<^sub>cG c2 (fresh S) s' n2" "n = n1 + n2"
+    by auto
+  from \<open>set (vars (If' b c1 c2)) \<subseteq> set S\<close> have "set (vars c1) \<subseteq> set S" "set (vars c2) \<subseteq> set S"
+    by simp+have "b \<in> set S" 
+     using \<open>set (vars (If' b c1 c2)) \<subseteq> set S\<close> by fastforce 
+   hence "s b \<noteq> 0" 
+     using \<open>s' = s on set S\<close> \<open>s' b \<noteq> 0\<close> by auto
+  from "4.IH"[OF \<open>size\<^sub>cG c1 (fresh S) s' n1 \<close> \<open>s' = s on set S\<close> \<open>set (vars c1) \<subseteq> set S\<close>] 
+  obtain t2 z2 where "(inline_S S c1, s) \<Rightarrow>\<^sub>G\<^bsup> z2 \<^esup> t2 " "t2 = t on set S " "C \<le> z2"
+    by auto 
+  from IfTrue[of s b "(inline_S S c1)" z2 t2 _ "(inline_S S c2)"]
+  have 1: "(If b (inline_S S c1) (inline_S S c2), s) \<Rightarrow>\<^sub>G\<^bsup> z2 + 1\<^esup> t2" 
+    using \<open>s b \<noteq> 0 \<close> \<open>(inline_S S c1, s) \<Rightarrow>\<^sub>G\<^bsup> z2 \<^esup> t2\<close>
+    by (simp add: big_step_tG.IfTrue)
+  have "Suc C \<le> Suc z2"
+    using \<open>C \<le> z2\<close> by auto
+  hence "C' \<le> Suc z2"
+    by (simp add: \<open>C' = Suc C\<close>)
+  hence "C' \<le> Suc z2"
+    by (auto simp: algebra_simps)
+  hence 3: "C' \<le> Suc z2"
+    using \<open>n = n1 + n2\<close> by auto
+  from 1 3  show ?case 
+    by (metis Suc_eq_plus1 \<open>t2 = t on set S\<close> inline_S.simps(4))
+next
+  case (5 s' b c2 C t C' c1)
+  from \<open>size\<^sub>cG (If' b c1 c2) (fresh S) s' n\<close> obtain n1 n2 x'  where
+      "size\<^sub>cG c1 (fresh S) s' n1""size\<^sub>cG c2 (fresh S) s' n2" "n = n1 + n2"
+    by auto
+  from \<open>set (vars (If' b c1 c2)) \<subseteq> set S\<close> have "set (vars c1) \<subseteq> set S" "set (vars c2) \<subseteq> set S"
+    by simp+have "b \<in> set S" 
+     using \<open>set (vars (If' b c1 c2)) \<subseteq> set S\<close> by fastforce 
+   hence "s b = 0" 
+     using \<open>s' = s on set S\<close> \<open>s' b = 0\<close> by auto
+  from "5.IH"[OF \<open>size\<^sub>cG c2 (fresh S) s' n2 \<close> \<open>s' = s on set S\<close> \<open>set (vars c2) \<subseteq> set S\<close>] 
+  obtain t2 z2 where "(inline_S S c2, s) \<Rightarrow>\<^sub>G\<^bsup> z2 \<^esup> t2 " "t2 = t on set S " "C \<le> z2"
+    by auto 
+  from IfFalse[of s b "(inline_S S c1)" z2 t2 _ "(inline_S S c2)"]
+  have 1: "(If b (inline_S S c1) (inline_S S c2), s) \<Rightarrow>\<^sub>G\<^bsup> z2 + 1\<^esup> t2" 
+    using \<open>s b = 0 \<close> \<open>(inline_S S c2, s) \<Rightarrow>\<^sub>G\<^bsup> z2 \<^esup> t2\<close>
+    by (simp add: big_step_tG.IfFalse)
+  have "Suc C \<le> Suc z2"
+    using \<open>C \<le> z2\<close> by auto
+  hence "C' \<le> Suc z2"
+    by (simp add: \<open>C' = Suc C\<close>)
+  hence "C' \<le> Suc z2"
+    by (auto simp: algebra_simps)
+  hence 3: "C' \<le> Suc z2"
+    using \<open>n = n1 + n2\<close> by auto
+  from 1 3  show ?case 
+    by (metis Suc_eq_plus1 \<open>t2 = t on set S\<close> inline_S.simps(4))
+next
+  case (6 s b c)
+  then show ?case sorry
+next
+  case (7 s1 b c C1 s2 C2 s3 C3)
+  from \<open>s1 b \<noteq> 0\<close> \<open>set (vars (While' b c)) \<subseteq> set S\<close> \<open> s1 = s on set S\<close> have \<open>s b \<noteq> 0\<close> by auto
+  from \<open>set (vars (While' b c)) \<subseteq> set S\<close> have \<open>set (vars c) \<subseteq> set S\<close> by auto
+  from \<open>size\<^sub>cG (While' b c) (fresh S) s1 n\<close> have \<open>size\<^sub>cG c (fresh S) s1 n\<close> by auto
+  obtain n2 where "size\<^sub>cG (While' b c) (fresh S) s2 n2"
+    using size\<^sub>cG_total by blast
+  from "7.IH"(1)[OF \<open>size\<^sub>cG c (fresh S) s1 n\<close> \<open>s1 = s on set S\<close> \<open>set (vars c) \<subseteq> set S\<close>]
+  obtain C1' s2' where 1: \<open>(inline_S S c, s) \<Rightarrow>\<^sub>G\<^bsup> C1' \<^esup> s2' \<close>\<open> s2' = s2 on set S \<close> \<open> C1' \<le> C1 + (C1 + 1) * n\<close> by auto
+  hence \<open>s2 = s2' on set S\<close> by auto
+  from "7.IH"(2)[OF \<open>size\<^sub>cG (While' b c) (fresh S) s2 n2\<close> \<open>s2 = s2' on set S\<close> \<open>set (vars (While' b c)) \<subseteq> set S\<close>]
+  obtain C2' s3' where 2: \<open>(inline_S S (While' b c), s2') \<Rightarrow>\<^sub>G\<^bsup> C2' \<^esup> s3' \<close>\<open> s3' = s3 on set S \<close> \<open> C2' \<le> C2 + (C2 + 1) * n2\<close>  by auto
+  hence \<open>((While b (inline_S S c)), s2') \<Rightarrow>\<^sub>G\<^bsup> C2' \<^esup> s3'\<close> by auto
+  from \<open>(inline_S S c, s) \<Rightarrow>\<^sub>G\<^bsup> C1' \<^esup> s2' \<close> \<open>((While b (inline_S S c)), s2') \<Rightarrow>\<^sub>G\<^bsup> C2' \<^esup> s3'\<close>  \<open>s b \<noteq> 0\<close>
+  have \<open>((While b (inline_S S c)), s) \<Rightarrow>\<^sub>G\<^bsup> C1' + C2' + 1 \<^esup> s3'\<close> 
+    by (simp add: big_step_tG.WhileTrue)
+  hence \<open>(inline_S S (While' b c), s)  \<Rightarrow>\<^sub>G\<^bsup> C1' + C2' + 1 \<^esup> s3'\<close> by auto    
+  from \<open>C1 \<le> C1'\<close> \<open>C2 \<le> C2'\<close> \<open>C1 + C2 + 1 = C3\<close> have "C3 \<le> C1' + C2' + 1" by simp 
+  from \<open>(inline_S S (While' b c), s)  \<Rightarrow>\<^sub>G\<^bsup> C1' + C2' + 1 \<^esup> s3'\<close> \<open> s3' = s3 on set S\<close> \<open>C3 \<le> C1' + C2' + 1\<close> show ?case
+    by auto
+next
+  case (8 c s' z t r)
+  hence prems: "s' = s on set (r # vars c)" "set (r # vars c) \<subseteq> set S" 
+    using eq_onI eq_on_subset vars_com'.simps(6) by fastforce+
+
+  then obtain zr tr where
+    inline: "(inline1 S c r, s) \<Rightarrow>\<^sub>G\<^bsup>  zr \<^esup> tr" "t r = tr r" 
+    "assign_costs (A (V r)) s + (ssubst_costs (fresh S) (s(fresh S r := s r)) (vars c) + z) +
+               assign_costs (A (V r)) t = zr"
+    using inline1_sound[OF \<open>(c, s') \<Rightarrow>\<^sub>G\<^bsup> z \<^esup> t\<close> \<open>s' = s on set (r # vars c)\<close> \<open>set (r # vars c) \<subseteq> set S\<close>] by auto
+  with "8.prems"(1) inline1_unchanged[OF inline(1) prems(2)] have "tr = s'(r := tr r) on set S"
+    using "8.prems"(2) fun_upd_apply by fastforce
+  with inline have " (inline_S S (Call' c r), s) \<Rightarrow>\<^sub>G\<^bsup>  zr \<^esup> tr \<and> tr = s'(r := t r) on set S \<and> z \<le> zr" by simp
+  then show ?case by blast
+qed
+
 
 lemma inline_S_complete:
   assumes "(inline_S S c',s) \<Rightarrow>\<^bsup>z\<^esup> t" "s= s' on set S" "set (vars c') \<subseteq> set S"
