IMP-/Step_Semantics_Cost_Generalization/Vars_for_GC.thy
@@ -1,132 +1,8 @@
-theory Vars_for_GC imports Big_StepT_Generalized_Cost_Final "../Eq_On"
+theory Vars_for_GC imports "../Vars" Big_StepT_Generalized_Cost_Final "../Eq_On"
+
 begin
-
-
 
 sledgehammer_params [provers = cvc4 verit z3 spass vampire zipperposition]
-
-class vars =
-  fixes vars :: "'a \<Rightarrow> vname list"
-
-class subst = vars +
-  fixes subst :: "(vname \<Rightarrow> vname) \<Rightarrow> 'a \<Rightarrow> 'a"
-  assumes subst_vars[simp]: "set (vars (subst m c)) = m ` set (vars c)"
-
-instantiation atomExp :: vars
-begin
-
-fun vars_atomExp :: "atomExp \<Rightarrow> vname list" where
-"vars_atomExp (V var) = [var]" |
-"vars_atomExp (N _) = []"
-
-instance ..
-
-end
-
-instantiation atomExp :: subst
-begin
-
-fun subst_atomExp :: "(vname \<Rightarrow> vname) \<Rightarrow> atomExp \<Rightarrow> atomExp" where
-"subst m (V var) = V (m var)" |
-"subst m (N n) = N n"
-
-instance
-proof (standard, goal_cases)
-  case (1 m c)
-  then show ?case by (induction c) auto
-qed
-
-end
-
-instantiation aexp :: vars
-begin
-
-fun vars_aexp :: "aexp \<Rightarrow> vname list" where
-"vars (A e) = vars e" |
-"vars (Plus e\<^sub>1 e\<^sub>2) = vars e\<^sub>1 @ vars e\<^sub>2" |
-"vars (Sub e\<^sub>1 e\<^sub>2) = vars e\<^sub>1 @ vars e\<^sub>2" |
-"vars (Parity e) = vars e" |
-"vars (RightShift e) = vars e"
-
-instance ..
-
-end
-
-instantiation aexp :: subst
-begin
-
-fun subst_aexp :: "(vname \<Rightarrow> vname) \<Rightarrow> aexp \<Rightarrow> aexp" where
-"subst m (A e) = A (subst m e)" |
-"subst m (Plus e\<^sub>1 e\<^sub>2) = Plus (subst m e\<^sub>1) (subst m e\<^sub>2)" |
-"subst m (Sub e\<^sub>1 e\<^sub>2) = Sub (subst m e\<^sub>1) (subst m e\<^sub>2)" |
-"subst m (Parity e) = Parity (subst m e)" |
-"subst m (RightShift e) = RightShift (subst m e)"
-
-instance
-proof (standard, goal_cases)
-  case (1 m c)
-  then show ?case by (induction c) auto
-qed
-
-end
-
-
-lemma atomVal_eq_if_eq_on_vars[simp]:
-  "s\<^sub>1 = s\<^sub>2 on set (vars a) \<Longrightarrow> atomVal a s\<^sub>1 = atomVal a s\<^sub>2"
-  by (induction a) auto
-
-lemma aval_eq_if_eq_on_vars [simp]:
-  "s\<^sub>1 = s\<^sub>2 on set (vars a) \<Longrightarrow> aval a s\<^sub>1 = aval a s\<^sub>2"
-  apply (induction a)
-  apply auto 
-  using atomVal_eq_if_eq_on_vars eq_on_subset
-  apply (metis sup.cobounded1 sup.cobounded2)+
-  done
-
-fun lvars :: "com \<Rightarrow> vname set" where
-"lvars SKIP = {}" |
-"lvars (x::=e) = {x}" |
-"lvars (c1;;c2) = lvars c1 \<union> lvars c2" |
-"lvars (IF b\<noteq>0 THEN c1 ELSE c2) = lvars c1 \<union> lvars c2" |
-"lvars (WHILE b\<noteq>0 DO c) = lvars c"
-
-instantiation com :: vars
-begin
-
-fun vars_com :: "com \<Rightarrow> vname list" where
-"vars SKIP = []" |
-"vars (x::=e) = x#vars e" |
-"vars (c1;;c2) = vars c1 @ vars c2" |
-"vars (IF b\<noteq>0 THEN c1 ELSE c2) = b # vars c1 @ vars c2" |
-"vars (WHILE b\<noteq>0 DO c) = b#vars c"
-
-instance ..
-
-end
-
-instantiation com :: subst
-begin
-
-fun subst_com :: "(vname \<Rightarrow> vname) \<Rightarrow> com \<Rightarrow> com" where
-"subst m SKIP = SKIP" |
-"subst m (x::=e) = (m x) ::= subst m e" |
-"subst m (c\<^sub>1;;c\<^sub>2) = subst m c\<^sub>1;; subst m c\<^sub>2" |
-"subst m (IF b\<noteq>0 THEN c\<^sub>1 ELSE c\<^sub>2) = IF m b\<noteq>0 THEN subst m c\<^sub>1 ELSE subst m c\<^sub>2" |
-"subst m (WHILE b\<noteq>0 DO c) = WHILE m b\<noteq>0 DO subst m c"
-
-instance
-proof (standard, goal_cases)
-  case (1 m c)
-  then show ?case by (induction c) auto
-qed
-
-end
-
-lemma atomVal_subst[simp]: "inj_on m (set (vars a)) \<Longrightarrow> atomVal (subst m a) s = (atomVal a (s o m))"
-  by (induction a) auto
-
-lemma aval_subst[simp]: "inj_on m (set (vars a)) \<Longrightarrow> aval (subst m a) s = aval a (s o m)"
-  by (induction a) (auto simp add: inj_on_Un)
 
 context BS_Generalized_Cost begin
 
@@ -164,6 +40,10 @@ lemma atom_Val_costs:
   apply (auto simp: subset_inj_on subsetD inj_on_contraD aval_eq_if_eq_on_vars[unfolded eq_on_def])
   by (induction a)  auto
 
+lemma atom_Val_cost_noninterference:
+ "set (vars a) \<subseteq> S \<Longrightarrow> s = s' on S \<Longrightarrow> atomVal_cost a s = atomVal_cost a s'"
+  by (induction a) auto
+  
 lemma aexp_costs: 
   "\<lbrakk> s = s' o m on S; set (vars a) \<subseteq> S; inj_on m S \<rbrakk>
     \<Longrightarrow>  aexp_cost (subst m a) s' = aexp_cost a s"unfolding eq_on_def
@@ -171,18 +51,24 @@ lemma aexp_costs:
   apply (induction a) apply auto
   by (metis atom_Val_costs comp_def eq_onI)+
 
+lemma aexp_costs_noninterference:
+ "set (vars a) \<subseteq> S \<Longrightarrow> s = s' on S \<Longrightarrow> aexp_cost a s = aexp_cost a s'"
+  using atom_Val_cost_noninterference by (induction a) auto
+
 lemma subst_costs_assign:
-  "\<lbrakk> s = s' o m on S; set (vars (x ::= a)) \<subseteq> S; inj_on m S \<rbrakk>
+  "\<lbrakk> s = s' o m on S; set (vars a) \<subseteq> S; inj_on m S \<rbrakk>
     \<Longrightarrow>  assign_costs (subst m a) s' = assign_costs a s" unfolding eq_on_def
   apply (auto simp: subset_inj_on subsetD inj_on_contraD aval_eq_if_eq_on_vars[unfolded eq_on_def])
   apply (induction a) apply auto
-  by (metis atom_Val_costs comp_eq_dest_lhs eq_onI)+
-  term "(m x) ::= subst m a"
+  sorry
+
+lemma assign_costs_noninterference:
+ "set (vars a) \<subseteq> S \<Longrightarrow> s = s' on S \<Longrightarrow> assign_costs a s = assign_costs a s'"
+  using atom_Val_cost_noninterference sorry
 
 lemma obtain_existing: 
   assumes "\<exists>t'. P t'"
   obtains t' where "P t'"
-  sledgehammer
   using assms by auto
 
 lemma subst_sound':
@@ -346,7 +232,7 @@ qed
 
 lemma subst_sound:
   "\<lbrakk> (c,s) \<Rightarrow>\<^sub>G\<^bsup>z\<^esup> t; s = s' o m on S; set (vars c) \<subseteq> S; inj_on m S \<rbrakk>
-    \<Longrightarrow> \<exists>t' z' . (subst m c,s') \<Rightarrow>\<^sub>G\<^bsup>z'\<^esup> t' \<and> t = t' o m on S"
+    \<Longrightarrow> \<exists>t' . (subst m c,s') \<Rightarrow>\<^sub>G\<^bsup>z\<^esup> t' \<and> t = t' o m on S"
   using subst_sound' subst_costs_unchanged by (metis big_step_t_state_determ2)
 
 lemma subst_complete':
@@ -401,11 +287,21 @@ lemma subst_complete:
     \<Longrightarrow> \<exists>t . (c,s) \<Rightarrow>\<^sub>G\<^bsup>z\<^esup> t \<and> t = t' o m on S"
   using subst_complete' subst_costs_unchanged  by (metis local.bigstep_det)
 
+
+lemma subst_id_atomVal: "subst id (c:: atomExp) = c"
+  by (cases c) auto
+
+corollary subst_id_aexp: "subst id (c::aexp) = c"
+  using subst_id_atomVal by (cases c)  auto
+
+corollary subst_id_com: "subst id (c::com) = c"
+  using subst_id_aexp by (induction c) auto
+
 lemma noninterference': 
   "(c,s) \<Rightarrow>\<^sub>G\<^bsup> x \<^esup> t \<Longrightarrow> set (vars c) \<subseteq> S \<Longrightarrow> s = s' on S \<Longrightarrow> \<exists>t' z'. (c,s') \<Rightarrow>\<^sub>G\<^bsup> z' \<^esup> t' \<and> t = t' on S"
 proof (induction c s x t arbitrary: s' rule: big_step_tG_induct)
   case (1 s)
-  then show ?case by auto 
+  then show ?case sorry
 next
   case (2 x a s)
   then show ?case unfolding eq_on_def
@@ -413,30 +309,43 @@ next
     by (metis "2.prems"(2) aval_eq_if_eq_on_vars big_step_tG.Assign eq_on_subset fun_upd_other fun_upd_same)
 next
   case (3 c1 s1 C1 s2 c2 C2 s3 C3)
-  then show ?case  unfolding eq_on_def
-    apply (auto simp: subset_inj_on subsetD inj_on_contraD aval_eq_if_eq_on_vars[unfolded eq_on_def])
-    sorry
+  have "set (vars c1) \<subseteq> S" and "set (vars c2) \<subseteq> S" using \<open>set (vars (c1;; c2)) \<subseteq> S\<close> by auto
+  have "\<exists>s2' z'. (((c1, s') \<Rightarrow>\<^sub>G\<^bsup> z' \<^esup> s2') \<and> s2 = s2'  on S)"
+    using \<open>s1 = s' on S\<close>  \<open>set (vars c1) \<subseteq> S\<close> "3.IH"(1)[of s']
+    by blast
+  then obtain s2' z' where 1: "(c1, s') \<Rightarrow>\<^sub>G\<^bsup> z' \<^esup> s2'" "s2 = s2' on S"    
+    by force
+  have "\<exists>t' z'. ((c2, s2') \<Rightarrow>\<^sub>G\<^bsup> z' \<^esup> t' \<and> s3 = t' on S)"
+    using \<open>s2 = s2' on S\<close>  \<open>set (vars c2) \<subseteq> S\<close> "3.IH"(2)[of s2']
+    by blast
+  with Seq obtain s3' z'' where 2: "(c2, s2')  \<Rightarrow>\<^sub>G\<^bsup> z'' \<^esup> s3'" "s3 = s3' on S" unfolding eq_on_def
+    by blast
+  let ?z''' = "z' + z''"
+  have "((c1;; c2), s') \<Rightarrow>\<^sub>G\<^bsup> ?z''' \<^esup> s3'"
+    using  1 2 Seq by auto
+  then show ?case unfolding eq_on_def using \<open>s3 = s3' on S\<close> 
+    by (metis "1"(1) "2"(1) "3.IH"(1) "3.IH"(2) "3.hyps"(3) "3.prems"(2) \<open>set (vars c1) \<subseteq> S\<close> \<open>set (vars c2) \<subseteq> S\<close> eq_onD local.bigstep_det)
 next
   case (4 s b c1 C t C' c2)
-  then show ?case sorry
+  then show ?case apply auto 
+    by (metis "4.hyps"(1) big_step_tG.IfTrue eq_on_def)
 next
   case (5 s b c2 C t C' c1)
-  then show ?case sorry
+  then show ?case apply auto 
+    by (metis big_step_tG.IfFalse eq_on_def)
 next
   case (6 s b c)
-  then show ?case sorry
+  then show ?case  apply auto 
+    by (metis big_step_tG.WhileFalse eq_on_def)
 next
   case (7 s1 b c C1 s2 C2 s3 C3)
-  then show ?case sorry
-qed
-  case (Assign x a s)
-  then show ?case 
-    using aval_eq_if_eq_on_vars big_step_t.Assign eq_on_def eq_on_subset fun_upd_apply set_subset_Cons vars_com.simps(2) by fastforce
-next
-  case (WhileTrue s1 b c x s2 y s3 z)
-  then show ?case apply auto
-    by (metis (mono_tags, lifting) WhileTrue.hyps(1) WhileTrue.hyps(4) big_step_t.WhileTrue eq_onE)
-qed fastforce+
+  then show ?case apply auto 
+    by (metis (mono_tags, lifting) "7.hyps"(1) big_step_tG.WhileTrue eq_onE)
+qed 
 
-
+lemma noninterference: 
+  "(c,s) \<Rightarrow>\<^sub>G\<^bsup> x \<^esup> t \<Longrightarrow> set (vars c) \<subseteq> S \<Longrightarrow> s = s' on S \<Longrightarrow> \<exists>t'. (c,s') \<Rightarrow>\<^sub>G\<^bsup> x \<^esup> t' \<and> t = t' on S"
+  using subst_complete[of id] subst_id_com 
+  by (smt (verit, ccfv_threshold) BS_Generalized_Cost.big_step_t_state_determ2 BS_Generalized_Cost_axioms comp_id inj_on_id subst_costs_unchanged)
+end
 end
