IMP-/Small_StepT.thy
@@ -17,6 +17,7 @@ Assign:  "(x ::= a, s) \<rightarrow> (SKIP, s(x := aval a s))" |
 Seq1:    "(SKIP;;c\<^sub>2,s) \<rightarrow> (c\<^sub>2,s)" |
 Seq2:    "(c\<^sub>1,s) \<rightarrow> (c\<^sub>1',s') \<Longrightarrow> (c\<^sub>1;;c\<^sub>2,s) \<rightarrow> (c\<^sub>1';;c\<^sub>2,s')" |
 
+IfTrue:  "s b \<noteq> 0 \<Longrightarrow> (IF b \<noteq>0 THEN c\<^sub>1 ELSE c\<^sub>2,s) \<rightarrow> (c\<^sub>1,s)" |
 IfFalse: "s b = 0 \<Longrightarrow> (IF b \<noteq>0  THEN c\<^sub>1 ELSE c\<^sub>2,s) \<rightarrow> (c\<^sub>2,s)" |
 
 WhileTrue:   "s b \<noteq> 0 \<Longrightarrow> (WHILE b\<noteq>0 DO c,s) \<rightarrow>
